add basic expr typechecking

C0deine/Type/Typ.lean
@@ -9,10 +9,10 @@ deriving DecidableEq, Inhabited, Hashable
 
 mutual
 inductive Typ
-| prim (prim : Typ.Primitive)
-| mem (mem : Typ.Memory)
+| prim (p : Typ.Primitive)
+| mem (m : Typ.Memory)
 | void_star
-| alias (sym : Symbol)
+| any
 deriving Inhabited, Hashable
 
 inductive Typ.Memory
@@ -22,12 +22,12 @@ inductive Typ.Memory
 deriving Inhabited, Hashable
 end
 
-namespace C0deine.Typ
+namespace Typ
 
 def Primitive.toString : Typ.Primitive → String
   | .int  => "int"
   | .bool => "bool"
-instance : ToString Typ.Primitive where toString := Typ.Primitive.toString
+instance : ToString Primitive where toString := Primitive.toString
 
 mutual
 def Memory.toString : Typ.Memory → String
@@ -36,16 +36,34 @@ def Memory.toString : Typ.Memory → String
   | .struct (sym : Symbol) => s!"struct {sym}"
 
 def toString : Typ → String
-  | .prim (prim : Typ.Primitive) => Typ.Primitive.toString prim
-  | .mem (mem : Typ.Memory) => Typ.Memory.toString mem
+  | prim (p : Primitive) => Primitive.toString p
+  | .mem (m : Typ.Memory) => Memory.toString m
   | .void_star => "void *"
-  | .alias (sym : Symbol) => s!"{sym}"
+  | .any => "'any"
 end
 
 instance : ToString Typ.Memory where toString := Typ.Memory.toString
 instance : ToString Typ where toString := Typ.toString
 
 mutual
+-- encoding structural equality
+def deq (a b : Typ) : Decidable (a = b) :=
+  match a, b with
+  | .prim p1, .prim p2 =>
+    match decEq p1 p2 with
+    | isTrue h  => isTrue  <| h ▸ rfl
+    | isFalse h => isFalse <| fun h' => by simp at h'; apply h h'
+  | .mem m1, .mem m2 =>
+    match Typ.Memory.deq m1 m2 with
+    | isTrue h  => isTrue  <| h ▸ rfl
+    | isFalse h => isFalse <| fun h' => by simp at h'; apply h h'
+  | .void_star, .void_star =>
+    isTrue <| Eq.refl Typ.void_star
+  | .any, .any =>
+    isTrue <| Eq.refl Typ.any
+  | _, _ => sorry
+    -- isFalse <| fun h => _
+
 def Memory.deq (a b : Typ.Memory) : Decidable (a = b) :=
   match a, b with
   | .struct s1, .struct s2 =>
@@ -62,32 +80,32 @@ def Memory.deq (a b : Typ.Memory) : Decidable (a = b) :=
     | isFalse h => isFalse <| fun h' => by simp at h'; apply h h'
   | _, _ => sorry
     -- isFalse <| _
-
-def deq (a b : Typ) : Decidable (a = b) :=
-  match a, b with
-  | .prim p1, .prim p2 =>
-    match decEq p1 p2 with
-    | isTrue h  => isTrue  <| h ▸ rfl
-    | isFalse h => isFalse <| fun h' => by simp at h'; apply h h'
-  | .mem m1, .mem m2 =>
-    match Typ.Memory.deq m1 m2 with
-    | isTrue h  => isTrue  <| h ▸ rfl
-    | isFalse h => isFalse <| fun h' => by simp at h'; apply h h'
-  | .void_star, .void_star =>
-    isTrue <| Eq.refl Typ.void_star
-  | .alias s1, .alias s2 =>
-    match decEq s1 s2 with
-    | isTrue h  => isTrue  <| h ▸ rfl
-    | isFalse h => isFalse <| fun h' => by simp at h'; apply h h'
-  | _, _ => sorry
-    -- isFalse <| fun h => _
-
 end
 
 instance : DecidableEq Typ.Memory := Typ.Memory.deq
 instance : DecidableEq Typ := Typ.deq
 
--- A type is reduced if it contains no aliases
+mutual
+  def equiv (a b : Typ) : Bool :=
+    match a, b with
+    | .prim p1  , .prim p2    => p1 == p2
+    | .mem m1   , .mem m2     => Memory.equiv m1 m2
+    | .void_star, .void_star  => true
+    | .any, _ | _, .any       => true
+    | _, _                    => false
+
+  def Memory.equiv (a b : Memory) : Bool :=
+    match a, b with
+    | .pointer t1, .pointer t2 => equiv t1 t2
+    | .array t1  , .array t2   => equiv t1 t2
+    | .struct s1 , .struct s2  => s1 == s2
+    | _, _                     => false
+end
+
+instance : BEq Typ where beq := equiv
+instance : BEq Memory where beq := Memory.equiv
+
+-- A type is reduced if it contains no "any"
 -- todo: do we need to lookup the symbol for structures?
 mutual
 inductive Reduced : Typ → Prop where
@@ -99,11 +117,10 @@ inductive Reduced : Typ → Prop where
 inductive Memory.Reduced : Memory → Prop where
 | pointer_reduced : ∀ t, Reduced t → Memory.Reduced (Typ.Memory.pointer t)
 | array_reduced   : ∀ t, Reduced t → Memory.Reduced (Typ.Memory.array t)
-| struct_reduced  : ∀ s, Memory.Reduced (Typ.Memory.Reduced s)
+| struct_reduced  : ∀ s, Memory.Reduced (Typ.Memory.struct s)
 end
 
-theorem Reduced.not_alias : ∀ s, ¬ Reduced (Typ.alias s) :=
-  fun _ => fun h => nomatch h
+theorem Reduced.not_any : ¬ Reduced (Typ.any) := fun h => nomatch h
 
 def isScalar : Typ → Bool
   | .prim .int => true
