C0deine/Type/Typechecker.lean
@@ -1,7 +1,338 @@
 import Std
 import C0deine.Parser.Ast
+import C0deine.Type.Typ
 import C0deine.Type.Tst
+import C0deine.Utils.Symbol
 import C0deine.Utils.Comparison
 
 namespace C0deine.Typechecker
 
+structure FuncType where
+  ret : Option Typ
+  args : List Typ
+
+structure Status.Var where
+  type : Typ
+  initialised : Bool
+
+structure Status.Func where
+  type : FuncType
+  defined : Bool
+
+structure Status.Struct where
+  fields : Symbol.Map Typ
+  defined : Bool
+
+inductive Status.Symbol
+| var (v : Status.Var)
+| func (f : Status.Func)
+| alias (type : Typ)
+
+def SymbolTable := Symbol.Map Status.Symbol
+def StructTable := Symbol.Map Status.Struct
+
+structure FuncCtx where
+  symbols : SymbolTable
+  structs : StructTable
+  ret_type : Option Typ
+  returns : Bool
+
+structure GlobalCtx where
+  symbols : SymbolTable
+  structs : StructTable
+
+
+def Trans.type (ctx : FuncCtx) : Ast.Typ → Option Typ
+  | .int => some <| Typ.prim (Typ.Primitive.int)
+  | .bool => some <| Typ.prim (Typ.Primitive.bool)
+  | .void => none
+  | .tydef name =>
+    match ctx.symbols.find? name with
+    | some (.alias tau) => some tau
+    | _ => none
+  | .ptr (.void) => some Typ.void_star
+  | .ptr (tau : Ast.Typ) =>
+    Trans.type ctx tau |>.map (Typ.mem ∘ Typ.Memory.pointer)
+  | .arr (tau : Ast.Typ) =>
+    Trans.type ctx tau |>.map (Typ.mem ∘ Typ.Memory.array)
+  | .struct name => some <| Typ.mem (Typ.Memory.struct name)
+
+def Trans.binop : Ast.BinOp → Tst.BinOp
+  | .int .plus  => .int .plus
+  | .int .minus => .int .minus
+  | .int .times => .int .times
+  | .int .div   => .int .div
+  | .int .mod   => .int .mod
+  | .int .and   => .int .and
+  | .int .xor   => .int .xor
+  | .int .or    => .int .or
+  | .int .lsh   => .int .lsh
+  | .int .rsh   => .int .rsh
+  | .cmp .lt    => .cmp .less
+  | .cmp .le    => .cmp .greater
+  | .cmp .gt    => .cmp .equal
+  | .cmp .ge    => .cmp .not_equal
+  | .cmp .eq    => .cmp .less_equal
+  | .cmp .ne    => .cmp .greater_equal
+  | .bool .and  => .bool .and
+  | .bool .or   => .bool .or
+
+
+
+-- todo: we should prove that these actually do what we want
+def Validate.var (ctx : FuncCtx)
+                 (var : Symbol)
+                 (tau : Typ)
+                 (initialised : Bool)
+                 : Except String FuncCtx := do
+  if ¬Typ.isSmall tau
+  then throw s!"Variable {var} must have a small type"
+  else
+    match ctx.symbols.find? var with
+    | some (.var _) => throw s!"Variable {var} is declared twice"
+    | some (.alias _) =>
+      throw s!"Variable {var} is declared but also used as a type alias"
+    | some (.func _) | none => -- allow shadowing of func declaration
+      return {ctx with symbols := ctx.symbols.insert var (.var ⟨tau, initialised⟩)}
+
+def Validate.typedef (ctx : FuncCtx)
+                     (var : Symbol)
+                     (tau : Typ)
+                     : Except String FuncCtx := do
+  if ctx.symbols.contains var
+  then throw s!"Name for typedef {var} already used"
+  else return {ctx with symbols := ctx.symbols.insert var (.alias tau)}
+
+def Validate.params (ctx : FuncCtx)
+                    (params : List Ast.Param)
+                    : Except String FuncCtx := do
+  match params with
+  | .nil => return ctx
+  | .cons p ps =>
+    match Trans.type ctx p.type with
+    | none     => throw "Function paramter has void or unknown type"
+    | some tau =>
+      let ctx' ← Validate.var ctx p.name tau true
+      Validate.params ctx' ps
+
+-- does not add function to the context!
+def Validate.func (ctx : FuncCtx)
+                  (name : Symbol)
+                  (inputs : List Ast.Param)
+                  (output : Option Typ)
+                  : Except String FuncCtx := do
+  if ctx.symbols.contains name
+  then throw s!"Name for function {name} already used"
+  else if ¬(output.all Typ.isSmall)
+  then throw s!"Function {name} must have small output type"
+  else Validate.params ctx inputs
+
+def Synth.ExprResult := Except String (Tst.Typed Tst.Expr)
+
+def Synth.binop_type (expect : Typ)
+                     (lhs : Typ)
+                     (rhs : Typ)
+                     : Except String Typ := do
+  let check := fun ty =>
+    if expect = ty
+    then pure ty
+    else throw "Binary operator is not well-typed"
+  match lhs, rhs with
+  | .prim .int, .prim .int
+  | .prim .int, .any
+  | .any, .prim .int          => check (.prim .int)
+  | .prim .bool, .prim .bool
+  | .prim .bool, .any
+  | .any, .prim .bool         => check (.prim .bool)
+  | .any, .any                => pure expect
+  | _, _ => throw "Binary operator is not well-typed"
+
+def Synth.intersect_types (tau1 tau2 : Typ) : Except String Typ := do
+  match tau1, tau2 with
+  | .any, _  => return tau2
+  | _ , .any => return tau1
+  | .prim .int, .prim .int
+  | .prim .bool, .prim .bool
+  | .void_star, .void_star   => return tau1
+  | .mem (.pointer tau1'), .mem (.pointer tau2')
+  | .mem (.array tau1'), .mem (.array tau2')     =>
+    Synth.intersect_types tau1' tau2'
+  | .mem (.struct s1), .mem (.struct s2) =>
+    if s1 = s2
+    then return tau1
+    else throw "Cannot intersect incompatible types"
+  | _, _ => throw "Cannot intersect incompatible types"
+
+mutual
+def Synth.expr (ctx : FuncCtx) (e : Ast.Expr) : Synth.ExprResult := do
+  match e with
+  | .num n             => return ⟨.prim (.int), .num n⟩
+  | .«true»            => return ⟨.prim (.bool), .«true»⟩
+  | .«false»           => return ⟨.prim (.bool), .«false»⟩
+  | .null              => return ⟨.mem (.pointer .any), .null⟩
+  | .unop op e         => Synth.unop ctx op e
+  | .binop op l r      => Synth.binop ctx op l r
+  | .ternop cond tt ff => Synth.ternop ctx cond tt ff
+  | .app f args        => Synth.app ctx f args
+  | .alloc ty          => Synth.alloc ctx ty
+  | .alloc_array ty e  => Synth.alloc_array ctx ty e
+  | .var name          => Synth.var ctx name
+  | .dot e field       => Synth.dot ctx e field
+  | .arrow e field     => Synth.arrow ctx e field
+  | .deref e           => Synth.deref ctx e
+  | .index e index     => Synth.index ctx e index
+
+def Synth.unop (ctx : FuncCtx)
+               (op : Ast.UnOp)
+               (e : Ast.Expr)
+               : Synth.ExprResult := do
+  let te ← Synth.expr ctx e
+  let (op', tau) ←
+    match op, te.typ with
+    | .int .neg, .prim .int
+    | .int .neg, .any         => pure (.int .neg, .prim .int)
+    | .int .not, .prim .int
+    | .int .not, .any         => pure (.int .not, .prim .int)
+    | .bool .neg, .prim .bool
+    | .bool .neg, .any        => pure (.bool .neg, .prim .bool)
+    | _, _ => throw "Unary operator is not well-typed"
+  return ⟨tau, .unop op' te⟩
+
+def Synth.binop (ctx : FuncCtx)
+                (op : Ast.BinOp)
+                (l r : Ast.Expr)
+                : Synth.ExprResult := do
+  let l' ← Synth.expr ctx l
+  let r' ← Synth.expr ctx r
+  let tau ←
+    match op with
+    | .int .plus
+    | .int .minus
+    | .int .times
+    | .int .div
+    | .int .mod
+    | .int .and
+    | .int .xor
+    | .int .or
+    | .int .lsh
+    | .int .rsh   => Synth.binop_type (.prim .int) l'.typ r'.typ
+    | .bool .and
+    | .bool .or
+    | .cmp .lt
+    | .cmp .le
+    | .cmp .gt
+    | .cmp .ge    => Synth.binop_type (.prim .bool) l'.typ r'.typ
+    | .cmp .eq
+    | .cmp .ne    =>
+      if l'.typ = r'.typ
+      then pure (.prim .bool)
+      else throw "Binary operator is not well-typed"
+  return ⟨tau, .binop (Trans.binop op) l' r'⟩
+
+def Synth.ternop (ctx : FuncCtx) (c tt ff : Ast.Expr) : Synth.ExprResult := do
+  let c' ← Synth.expr ctx c
+  let tt' ← Synth.expr ctx tt
+  let ff' ← Synth.expr ctx ff
+  if c'.typ ≠ .prim .bool
+  then throw "Ternary condition must be a bool"
+  else
+    let tau ← Synth.intersect_types tt'.typ ff'.typ
+    return ⟨tau, .ternop c' tt' ff'⟩
+
+def Synth.app (ctx : FuncCtx)
+              (f : Ast.Ident)
+              (args : List Ast.Expr)
+              : Synth.ExprResult := do
+  match ctx.symbols.find? f with
+  | some (.func status) =>
+    let args' ← args.mapM (Synth.expr ctx)
+    let arg_types := args'.map (fun arg => arg.typ)
+    let ret_type := -- return unit (i.e. void_star) if there's no return type
+      match status.type.ret with
+      | some tau => tau
+      | none => .void_star
+    if arg_types == status.type.args
+    then return ⟨ret_type, .app f args'⟩
+    else throw "Function argument types don't match"
+  | _ => throw "Cannot apply to a non-function type"
+
+def Synth.alloc (ctx : FuncCtx) (tau : Ast.Typ) : Synth.ExprResult := do
+  let opt_tau' := Trans.type ctx tau
+  match opt_tau' with
+  | some tau' => return ⟨.mem (.pointer tau'), .alloc tau'⟩
+  | none      => throw s!"Invalid allocation type"
+
+def Synth.alloc_array (ctx : FuncCtx)
+                      (tau : Ast.Typ)
+                      (e : Ast.Expr)
+                      : Synth.ExprResult := do
+  let opt_tau' := Trans.type ctx tau
+  let e' ← Synth.expr ctx e
+  match opt_tau', e'.typ with
+  | none, _ => throw s!"Invalid array type"
+  | some tau', .prim .int => return ⟨.mem (.array tau'), .alloc_array tau' e'⟩
+  | _, _ => throw "Array length must be an integer"
+
+def Synth.var (ctx : FuncCtx) (var : Ast.Ident) : Synth.ExprResult := do
+  match ctx.symbols.find? var with
+  | some (.var status) =>
+    if status.initialised
+    then return ⟨status.type, .var var⟩
+    else throw s!"Variable {var} not initialised"
+  | _ => throw s!"Variable {var} not declared"
+
+def Synth.dot (ctx : FuncCtx)
+              (e : Ast.Expr)
+              (field : Ast.Ident)
+              : Synth.ExprResult := do
+  let e' ← Synth.expr ctx e
+  match e'.typ with
+  | .mem (.pointer <| .mem (.struct name)) =>
+    match ctx.structs.find? name with
+    | some status =>
+      if ¬status.defined
+      then throw s!"Struct {name} is not defined"
+      else
+        match status.fields.find? field with
+        | some tau => return ⟨tau, .dot e' field⟩
+        | none => throw s!"Invalid field {field}}"
+    | none => throw s!"Struct {name} is not defined"
+  | _ => throw s!"Arrow operator must be used on a struct pointer"
+
+def Synth.arrow (ctx : FuncCtx)
+                (e : Ast.Expr)
+                (field : Ast.Ident)
+                : Synth.ExprResult := do
+  let e' ← Synth.expr ctx e
+  match e'.typ with
+  | .mem (.struct name) =>
+    match ctx.structs.find? name with
+    | some status =>
+      if ¬status.defined
+      then throw s!"Struct {name} is not defined"
+      else
+        match status.fields.find? field with
+        | some tau => return ⟨tau, .dot e' field⟩
+        | none => throw s!"Invalid field {field}}"
+    | none => throw s!"Struct {name} is not defined"
+  | _ => throw s!"Field accessor can only operate on a struct"
+
+def Synth.deref (ctx : FuncCtx) (e : Ast.Expr) : Synth.ExprResult := do
+  let e' ← Synth.expr ctx e
+  match e'.typ with
+  | .mem (.pointer .any) => throw "Cannot dereference a null pointer/function"
+  | .mem (.pointer tau)  => return ⟨tau, .deref e'⟩
+  | _ => throw "Cannot dereference a non-pointer type"
+
+def Synth.index (ctx : FuncCtx)
+                (arr : Ast.Expr)
+                (index : Ast.Expr)
+                : Synth.ExprResult := do
+  let arr' ← Synth.expr ctx arr
+  let index' ← Synth.expr ctx index
+  match arr'.typ, index'.typ with
+  | .mem (.array tau), .prim .int => return ⟨tau, .index arr' index'⟩
+  | .mem (.array tau), _ => throw "Array indices must be integers"
+  | _, _ => throw "Indexing can only be done on array types"
+
+end
