C0deine/utils/Symbol.lean
@@ -9,3 +9,6 @@ deriving DecidableEq, Inhabited
 
 instance : ToString Symbol where toString | s => s.name
 instance : Hashable Symbol where hash | s => s.id
+
+universe u
+def Symbol.Map (α : Type u) := Std.HashMap Symbol α
